\centering
\setlength{\columnsep}{-1cm}
\begin{multicols}{2}
	\begin{mgrammar}
		\firstrule{r}{\tau}{}
		\grule{T}{}
		\gskip
		\firstrule{\tau}{\pi}{}
		\grule{\phi}{}
		\grule{\bar{\tau}}{}
		\gskip
		\firstrule{\pi}{\scalar{r, r}}{}
		\gskip
		\firstrule{\phi}{r \to r}{}
		\gskip
		\firstrule{\bar{\tau}}{\e}{}
		\grule{\t}{}
		\grule{\vdots}{}
		\gskip
		\firstrule{T}{F \tau}{}
		\gskip
		\firstrule{F}{\mathcal{F}\left(\mL\right)^{*}}{}
		\gskip
	\end{mgrammar}

	\begin{mgrammar}
		\firstrule{\text{Tree}}{\tau, \tau}{}
		\gskip
		\firstrule{\text{SM}}{\combML \enspace|\enspace \combMR}{\fmap}
		\grule{\combUL \enspace|\enspace \combUR}{\tt pure}
		\grule{\combA}{\tt Struct}
		\grule{\combJ}{\tt join}
		\grule{\combC}{\tt counit}
		\grule{\combER \enspace|\enspace \combEL}{\tt eject}
		\grule{\combDN}{\tt closure}
		\gskip
		\firstrule{\text{M}}{\text{SM}, \text{M}}{}
		\grule{\text{BComb}}{}
		\gskip
		\firstrule{\text{BComb}}{\mathrm{>} \enspace|\enspace \mathrm{<} \enspace|\enspace \wedge \enspace|\enspace \vee}{}
	\end{mgrammar}
\end{multicols}

\def\arraystretch{1.5}
\begin{mgrammar}
	\firstrule{\combMR_{\f{F}} (\alpha, \beta)}{\f{F}\alpha, \beta}{}
	\firstrule{\combML_{\f{F}} (\alpha, \beta)}{\alpha, \f{F}\beta}{}
	\firstrule{\combA_{\f{F}} (\alpha, \beta)}{\f{F}\alpha, \f{F}\beta}{}
	\firstrule{\combUR_{\f{F}} (\alpha \to \alpha', \beta)}{\f{F}\alpha\to \alpha', \beta}{}
	\firstrule{\combUL_{\f{F}} (\alpha, \beta\to \beta')}{\alpha, \f{F}\beta \to \beta'}{}
	\firstrule{\combC_{\f{L}\f{R}} (\f{L} \alpha, \f{R}\beta)}{(\alpha, \beta)}{}
	\firstrule{\combER_{\f{R}} (\f{R}(\alpha \to \alpha'), \beta)}{\alpha\to \f{R}\alpha', \beta}{}
	\firstrule{\combEL_{\f{R}} (\alpha, \f{R}(\beta \to \beta'))}{\alpha, \beta\to \f{R}\beta'}{}
	\gskip
	\firstrule{>, \beta}{(\alpha\to \beta), \alpha}{}
	\firstrule{<, \beta}{\alpha, (\alpha \to \beta)}{}
	\firstrule{\wedge, \alpha \to \t}{(\alpha \to \t), (\alpha \to \t)}{}
	\firstrule{\vee, \alpha \to \t}{(\alpha \to \t), (\alpha \to \t)}{}
	\gskip
	\firstrule{\combJ_{\f{F}} \f{F}\tau}{\f{F}\f{F}\tau}{}
	\firstrule{\combDN_{\f{C}} \tau}{\f{C}_{\tau}\tau}{}
\end{mgrammar}

\medskip

\begin{mgrammar}
	\firstrule{\sobj}{M, r}{}
\end{mgrammar}

\medskip

\def\arraystretch{1.2}
\begin{mgrammar}
	\firstrule{\combMR_{\f{F}} M, \f{F}\alpha \to \beta \to \f{F}\gamma}{M, \alpha \to \beta \to \gamma}{}
	\firstrule{\combML_{\f{F}} M, \alpha \to \f{F}\beta \to \f{F}\gamma}{M, \alpha \to \beta \to \gamma}{}
	\firstrule{\combA_{\f{F}} M, \f{F}\alpha \to \f{F}\beta \to \f{F}\gamma}{M, \alpha \to \beta \to \gamma}{}
	\firstrule{\combUR_{\f{F}} M, \alpha \to (\f{F}\beta \to \beta') \to \gamma}{M, \alpha \to (\beta \to \beta') \to \gamma}{}
	\firstrule{\combUL_{\f{F}} M, (\f{F}\beta \to \beta') \to \alpha \to \gamma}{M, (\beta \to \beta') \to \alpha \to \gamma}{}
	\firstrule{\combJ_{\f{F}} M, \alpha \to \beta \to \f{F}\gamma}{M, \alpha \to \beta \f{F}\f{F}\gamma}{}
	\firstrule{\combC_{\f{L}\f{R}} M, \f{L}\alpha \to \f{R}\beta \to \gamma}{M, \alpha \to \beta \to \gamma}{}
	\firstrule{\combER_{\f{R}} M, (\alpha \to \f{R}\alpha') \to \beta \to \gamma}{M, \f{R}(\alpha \to \alpha')  \to \beta \to \gamma}{}
	\firstrule{\combEL_{\f{R}} M, \alpha \to (\beta \to \f{R}\beta') \to \gamma}{M, \alpha \to \f{R}(\beta \to \beta') \to \gamma}{}
	\firstrule{\combDN_{\f{C}} M, \alpha \to \beta \to \gamma}{\alpha \to \beta \to \f{C}_{\gamma}\gamma}{}
\end{mgrammar}
