\def\arraystretch{1.5}
% f Â· x = (\fmap_{\f{F}} f) (x)
% \eta = pure 
\begin{tabular}{R@{$=$}L}
	>               & \lambda \phi. \lambda x. \phi x                                            \\
	<               & \lambda x. \lambda \phi. \phi x                                            \\
	                &                                                                            \\
	\combML_{\f{F}} & \lambda M. \lambda \f{F}x. \lambda y. \fmap_{\f{F}} (\lambda a. M(a, y)) x \\
	\combMR_{\f{F}} & \lambda M. \lambda x. \lambda \f{F}y. \fmap_{\f{F}} (\lambda a. M(a, y)) x \\
	\combA_{\f{F}}  & \lambda M. \lambda \f{F}x. \lambda \f{F}y. \fmap_{\f{F}} M(x, y)
\end{tabular}
